{
 "cells": [
  {
   "cell_type": "code",
   "execution_count": 1,
   "metadata": {
    "collapsed": false
   },
   "outputs": [
    {
     "data": {
      "text/html": [
       "<script>\n",
       "code_show=true; \n",
       "function code_toggle() {\n",
       " if (code_show){\n",
       " $('div.input').hide();\n",
       " } else {\n",
       " $('div.input').show();\n",
       " }\n",
       " code_show = !code_show\n",
       "} \n",
       "$( document ).ready(code_toggle);\n",
       "</script>\n",
       "<form action=\"javascript:code_toggle()\"><input type=\"submit\" value=\"Click here to toggle on/off the raw code.\"></form>"
      ],
      "text/plain": [
       "<IPython.core.display.HTML object>"
      ]
     },
     "execution_count": 1,
     "metadata": {},
     "output_type": "execute_result"
    }
   ],
   "source": [
    "from IPython.display import HTML\n",
    "\n",
    "HTML('''<script>\n",
    "code_show=true; \n",
    "function code_toggle() {\n",
    " if (code_show){\n",
    " $('div.input').hide();\n",
    " } else {\n",
    " $('div.input').show();\n",
    " }\n",
    " code_show = !code_show\n",
    "} \n",
    "$( document ).ready(code_toggle);\n",
    "</script>\n",
    "<form action=\"javascript:code_toggle()\"><input type=\"submit\" value=\"Click here to toggle on/off the raw code.\"></form>''')"
   ]
  },
  {
   "cell_type": "markdown",
   "metadata": {},
   "source": [
    "### Solutions to the exercises set 1"
   ]
  },
  {
   "cell_type": "markdown",
   "metadata": {},
   "source": [
    "#### Exercise 1. Statistical independence implies zero covarience "
   ]
  },
  {
   "cell_type": "markdown",
   "metadata": {},
   "source": [
    "$X$ and $Y$ are independent so joint probability density $p(x,y) $ is equal to the product of marginal probability densities $p(x)$ and $p(y)$. \n",
    "$$p(x,y) = p(x)p(y)$$"
   ]
  },
  {
   "cell_type": "code",
   "execution_count": 20,
   "metadata": {
    "collapsed": false
   },
   "outputs": [
    {
     "data": {
      "text/latex": [
       "\\begin{equation}\n",
       "p(x,y) = p(x)p(y) \\\\\n",
       "cov(X,Y) = \\mathbb{E}[(X-\\mathbb{E}X)(Y-\\mathbb{E}Y)]=\\mathbb{E}[XY]-\\mathbb{E}[X]\\mathbb{E}[Y] \\\\\n",
       "\\mathbb{E}[XY] = \\int x\\cdot y \\cdot p(x,y)dxdy = \\int x\\cdot y \\cdot p(x)p(y)dxdy=\\int x\\cdot p(x)dx \\cdot \\int y\\cdot p(y)dy =\\mathbb{E}[X]\\mathbb{E}[Y]  \n",
       "\n",
       "\\end{equation}"
      ],
      "text/plain": [
       "<IPython.core.display.Latex object>"
      ]
     },
     "metadata": {},
     "output_type": "display_data"
    }
   ],
   "source": [
    "%%latex\n",
    "\\begin{equation}\n",
    "cov(X,Y) = \\mathbb{E}[(X-\\mathbb{E}X)(Y-\\mathbb{E}Y)]=\\mathbb{E}[XY]-\\mathbb{E}[X]\\mathbb{E}[Y] \\\\\n",
    "\\mathbb{E}[XY] = \\int x\\cdot y \\cdot p(x,y)dxdy = \\int x\\cdot y \\cdot p(x)p(y)dxdy=\\int x\\cdot p(x)dx \\cdot \\int y\\cdot p(y)dy =\\mathbb{E}[X]\\mathbb{E}[Y]  \n",
    "\\end{equation}"
   ]
  },
  {
   "cell_type": "markdown",
   "metadata": {},
   "source": [
    "For discrete variables the proof is similar, we just need to use sums, not integrals  "
   ]
  },
  {
   "cell_type": "markdown",
   "metadata": {},
   "source": [
    "#### Exercise 2. Probability calculus with apples and oranges "
   ]
  },
  {
   "cell_type": "markdown",
   "metadata": {},
   "source": [
    "1) We can use product rule. $$P(F=Apple)= P(F=Apple|Box= 1) \\cdot (Box = 1)+P(F=Apple|Box = 0) \\cdot (Box = 0)= \\frac{8}{12}\\cdot\\frac{1}{2}+\\frac{15}{18}\\cdot\\frac{1}{2}=0.75$$\n",
    "2) $$P(B = 1|F=A) = \\frac{ P(F= A|B = 1) \\cdot (B= 1)}{P(F=A)}= \\frac{4}{9}$$\n",
    "3) We don't know what the box is but we do know the probability of the box to be the first box or the second (we've just calculated them in 2). So we can once more use the product rule to find the probability that the second fruit is an apple. $$P(F2=A|F=A)= P(F2=A|B= 1) \\cdot (B= 1|F=A)+  P(F2=A|B = 0)  \\cdot (B = 0|F=A) = \\frac{8}{12}\\cdot\\frac{4}{9}+\\frac{15}{18}\\cdot(1-\\frac{4}{9})= 0.759$$"
   ]
  },
  {
   "cell_type": "code",
   "execution_count": 4,
   "metadata": {
    "collapsed": false
   },
   "outputs": [
    {
     "data": {
      "text/plain": [
       "0.7592592592592593"
      ]
     },
     "execution_count": 4,
     "metadata": {},
     "output_type": "execute_result"
    }
   ],
   "source": [
    "41/54"
   ]
  },
  {
   "cell_type": "code",
   "execution_count": 22,
   "metadata": {
    "collapsed": false
   },
   "outputs": [
    {
     "data": {
      "text/plain": [
       "0.75"
      ]
     },
     "execution_count": 22,
     "metadata": {},
     "output_type": "execute_result"
    }
   ],
   "source": [
    "(8/12+15/18)*(1/2)"
   ]
  },
  {
   "cell_type": "code",
   "execution_count": 5,
   "metadata": {
    "collapsed": false
   },
   "outputs": [
    {
     "data": {
      "text/plain": [
       "0.4444444444444444"
      ]
     },
     "execution_count": 5,
     "metadata": {},
     "output_type": "execute_result"
    }
   ],
   "source": [
    "(8/12)*(1/2)/(0.75)"
   ]
  },
  {
   "cell_type": "code",
   "execution_count": 27,
   "metadata": {
    "collapsed": false
   },
   "outputs": [
    {
     "data": {
      "text/plain": [
       "0.7592592592592593"
      ]
     },
     "execution_count": 27,
     "metadata": {},
     "output_type": "execute_result"
    }
   ],
   "source": [
    "(8/12)*(4/9)+(15/18)*(5/9)"
   ]
  },
  {
   "cell_type": "markdown",
   "metadata": {},
   "source": [
    "#### Exercise 3. Maximum likelihood "
   ]
  },
  {
   "cell_type": "code",
   "execution_count": 1,
   "metadata": {
    "collapsed": false,
    "scrolled": false
   },
   "outputs": [
    {
     "data": {
      "text/latex": [
       "1) We use a property that of the logarithm of product is equal to the sum of the logarithms\n",
       "\\begin{equation}\n",
       "\\log (p(\\chi|\\mu,\\sigma^2)) = \\log(\\prod_{i=1}^{N} \\mathcal{N}(x_n|\\mu,\\sigma^2)) = \\sum_{i=1}^{N} \\log (\\mathcal{N}(x_n|\\mu,\\sigma^2)))\\\\\n",
       "\\sum_{i=1}^{N} \\log \\mathcal{N}(x_n|\\mu,\\sigma^2) = \\sum_{i=1}^{N} \\log \\frac{1}{\\sqrt{2\\pi\\sigma^2}}e^{-\\frac{(x_n - \\mu)^2}{2\\sigma^2}} =\\\\\n",
       "= \\sum_{i=1}^{N} -\\frac{(x_n - \\mu)^2}{2\\sigma^2} + \\sum_{i=1}^{N} - \\frac{1}{2}\\log 2\\pi\\sigma^2 = \\\\ \n",
       "= -\\frac{1}{2\\sigma^2} \\sum_{i=1}^{N}(x_n - \\mu)^2 - \\frac{N}{2} \\log(\\sigma^2 ) - \\frac{N}{2} \\log(2\\pi)\n",
       "\\end{equation}\n",
       "2)\n",
       "\\begin{equation}\n",
       "\\frac{d \\log (p(\\chi|\\mu,\\sigma^2))}{d \\mu} = 0 \\\\\n",
       "\\frac{d \\log (p(\\chi|\\mu,\\sigma^2))}{d \\mu} = \\frac{2}{2\\sigma^2} \\sum_{i=1}^{N}(x_n - \\mu) =0 \\\\\n",
       "\\sum_{i=1}^{N} \\mu = \\sum_{i=1}^{N} x_n \\\\\n",
       "\\mu_{ML} = \\frac{1}{N}  \\sum_{i=1}^{N} x_n\n",
       "\\end{equation}\n",
       "3) \n",
       "\\begin{equation}\n",
       "\\frac{d \\log (p(\\chi|\\mu,\\sigma^2))}{d \\sigma^2} = 0 \\\\\n",
       "\\frac{d \\log (p(\\chi|\\mu,\\sigma^2))}{d \\sigma^2} = \\frac{1}{\\sigma^3}\\sum_{i=1}^{N}(x_n - \\mu)^2 -\\frac{N}{2}\\frac{1}{\\sigma^2}2\\sigma =0 \\\\\n",
       "\\sigma_{ML}^2 = \\frac{1}{N}\\sum_{i=1}^{N}(x_n - \\mu_{ML})^2\n",
       "\\end{equation}"
      ],
      "text/plain": [
       "<IPython.core.display.Latex object>"
      ]
     },
     "metadata": {},
     "output_type": "display_data"
    }
   ],
   "source": [
    "%%latex \n",
    "1) We use a property that of the logarithm of product is equal to the sum of the logarithms\n",
    "\\begin{equation}\n",
    "\\log (p(\\chi|\\mu,\\sigma^2)) = \\log(\\prod_{i=1}^{N} \\mathcal{N}(x_n|\\mu,\\sigma^2)) = \\sum_{i=1}^{N} \\log (\\mathcal{N}(x_n|\\mu,\\sigma^2)))\\\\\n",
    "\\sum_{i=1}^{N} \\log \\mathcal{N}(x_n|\\mu,\\sigma^2) = \\sum_{i=1}^{N} \\log \\frac{1}{\\sqrt{2\\pi\\sigma^2}}e^{-\\frac{(x_n - \\mu)^2}{2\\sigma^2}} =\\\\\n",
    "= \\sum_{i=1}^{N} -\\frac{(x_n - \\mu)^2}{2\\sigma^2} + \\sum_{i=1}^{N} - \\frac{1}{2}\\log 2\\pi\\sigma^2 = \\\\ \n",
    "= -\\frac{1}{2\\sigma^2} \\sum_{i=1}^{N}(x_n - \\mu)^2 - \\frac{N}{2} \\log(\\sigma^2 ) - \\frac{N}{2} \\log(2\\pi)\n",
    "\\end{equation}\n",
    "2)\n",
    "\\begin{equation}\n",
    "\\frac{d \\log (p(\\chi|\\mu,\\sigma^2))}{d \\mu} = 0 \\\\\n",
    "\\frac{d \\log (p(\\chi|\\mu,\\sigma^2))}{d \\mu} = \\frac{2}{2\\sigma^2} \\sum_{i=1}^{N}(x_n - \\mu) =0 \\\\\n",
    "\\sum_{i=1}^{N} \\mu = \\sum_{i=1}^{N} x_n \\\\\n",
    "\\mu_{ML} = \\frac{1}{N}  \\sum_{i=1}^{N} x_n\n",
    "\\end{equation}\n",
    "3) \n",
    "\\begin{equation}\n",
    "\\frac{d \\log (p(\\chi|\\mu,\\sigma^2))}{d \\sigma^2} = 0 \\\\\n",
    "\\frac{d \\log (p(\\chi|\\mu,\\sigma^2))}{d \\sigma^2} = \\frac{1}{\\sigma^3}\\sum_{i=1}^{N}(x_n - \\mu)^2 -\\frac{N}{2}\\frac{1}{\\sigma^2}2\\sigma =0 \\\\\n",
    "\\sigma_{ML}^2 = \\frac{1}{N}\\sum_{i=1}^{N}(x_n - \\mu_{ML})^2\n",
    "\\end{equation}"
   ]
  },
  {
   "cell_type": "markdown",
   "metadata": {},
   "source": [
    "#### Exercise 4 "
   ]
  },
  {
   "cell_type": "markdown",
   "metadata": {},
   "source": [
    "It is well-known [Boy or Girl \"paradox\"](https://en.wikipedia.org/wiki/Boy_or_Girl_paradox). Read part \"Analysis of the ambiguity\" to understand the difference between first that second situation. \n",
    "> Thus, if it is assumed that **both children were considered while looking for a boy**, the answer is \n",
    "**$\\frac{1}{3}$**. However, if the family was first selected and then **a random, true statement was made about the gender of one child** in that family, whether or not both were considered, the correct way to calculate the conditional probability is not to count all of the cases that include a child with that gender. Instead, one must consider only the probabilities where the statement will be made in each case. In this case the answer is **$\\frac{1}{2}$**."
   ]
  },
  {
   "cell_type": "markdown",
   "metadata": {},
   "source": [
    "#### Exercise 5"
   ]
  },
  {
   "cell_type": "code",
   "execution_count": 2,
   "metadata": {
    "collapsed": false
   },
   "outputs": [
    {
     "data": {
      "text/latex": [
       "\n",
       "\\begin{equation}\n",
       "p(x|\\mu,\\sigma^2)= \\frac{1}{\\sqrt{2\\pi\\sigma^2}}e^{-\\frac{(x - \\mu)^2}{2\\sigma^2}}\n",
       "\\end{equation}\n",
       "\n",
       "\\begin{equation}\n",
       "H[x] = - \\mathbb{E} [\\log p(x|\\mu,\\sigma^2)] = -(-\\frac{1}{2} \\log 2\\pi\\sigma^2 + \\mathbb{E}[-\\frac{(x - \\mu)^2}{2\\sigma^2}]) \\\\\n",
       "= \\frac{1}{2} \\log 2\\pi\\sigma^2 + \\frac{1}{2\\sigma^2}\\mathbb{E}[(x - \\mu)^2] = \\frac{1}{2}(\\log 2\\pi\\sigma^2+1)\n",
       "\\end{equation}"
      ],
      "text/plain": [
       "<IPython.core.display.Latex object>"
      ]
     },
     "metadata": {},
     "output_type": "display_data"
    }
   ],
   "source": [
    "%%latex \n",
    "\n",
    "\\begin{equation}\n",
    "p(x|\\mu,\\sigma^2)= \\frac{1}{\\sqrt{2\\pi\\sigma^2}}e^{-\\frac{(x - \\mu)^2}{2\\sigma^2}}\n",
    "\\end{equation}\n",
    "\n",
    "\\begin{equation}\n",
    "H[x] = - \\mathbb{E} [\\log p(x|\\mu,\\sigma^2)] = -(-\\frac{1}{2} \\log 2\\pi\\sigma^2 + \\mathbb{E}[-\\frac{(x - \\mu)^2}{2\\sigma^2}]) \\\\\n",
    "= \\frac{1}{2} \\log 2\\pi\\sigma^2 + \\frac{1}{2\\sigma^2}\\mathbb{E}[(x - \\mu)^2] = \\frac{1}{2}(\\log 2\\pi\\sigma^2+1)\n",
    "\\end{equation}\n"
   ]
  },
  {
   "cell_type": "code",
   "execution_count": null,
   "metadata": {
    "collapsed": true
   },
   "outputs": [],
   "source": []
  }
 ],
 "metadata": {
  "kernelspec": {
   "display_name": "Python 3",
   "language": "python",
   "name": "python3"
  },
  "language_info": {
   "codemirror_mode": {
    "name": "ipython",
    "version": 3
   },
   "file_extension": ".py",
   "mimetype": "text/x-python",
   "name": "python",
   "nbconvert_exporter": "python",
   "pygments_lexer": "ipython3",
   "version": "3.6.0"
  }
 },
 "nbformat": 4,
 "nbformat_minor": 2
}
